QI_Checker/Instantiation/subst.lean
@@ -2,7 +2,7 @@ import QI_Checker.IR.TermType
 import QI_Checker.IR.Term
 import QI_Checker.IR.Op
 
-open IR
+namespace IR.Term
 
 /-- Append an element to a substitution or a renaming.
 ```
@@ -33,8 +33,11 @@ theorem upr_id : upr id = id := by
   ext ⟨⟩ <;> dsimp [upr, snoc]
 
 /-- Rename the de Bruijn indices in an expression. -/
-def rename (ξ : Nat → Nat) : Term → Term :=
-  sorry
+def rename (ξ : Nat → Nat) : Term → Term
+  | .prim p => .prim p
+  | .var v => .var (ξ v)
+  | .app op args => .app op (List.map (rename ξ) args)
+  | .quant q bv body => .quant q bv (body.rename (upr ξ))
 
 /-! ## Substitution -/
 
@@ -53,19 +56,28 @@ def up (σ : Nat → Term) : Nat → Term :=
 
 @[simp]
 theorem up_var : up Term.var = Term.var := by
-  ext ⟨⟩ <;> (unfold up; dsimp [snoc, rename]); sorry
+  ext ⟨⟩ <;> (unfold up; simp [snoc, rename])
 
 /-- Apply a substitution to a term. -/
-def subst (σ : Nat → Term) : Term → Term := sorry
-
+def subst (σ : Nat → Term) : Term → Term
+  | .prim p => .prim p
+  | .var v => σ v
+  | .app op args => .app op (List.map (subst σ) args)
+  | .quant q bv body => .quant q bv (body.subst (up σ))
 
 @[simp]
-theorem subst_bvar: subst Term.var = id := by sorry
-  --ext t; dsimp; induction t <;> grind [subst, up_bvar]
+theorem map_id''_mem {f : α → α} (l : List α) (h : ∀ x ∈ l, f x = x)  : List.map f l = l := by
+  induction l
+  all_goals grind
+
+@[simp]
+theorem subst_var: subst Term.var = id := by
+  ext t; dsimp; induction t <;> simp [subst, up_var];
+  all_goals grind[map_id''_mem]
 
 @[simp]
 theorem subst_snoc_zero (σ : Nat → Term) (t : Term) : subst (snoc σ t) (.var 0) = t := by
-  dsimp [subst, snoc]; sorry
+  simp [subst, snoc]
 
 /-- Turn a renaming into a substitution. -/
 def ofRen (ξ : Nat → Nat) : Nat → Term :=
@@ -75,13 +87,13 @@ def ofRen (ξ : Nat → Nat) : Nat → Term :=
 theorem ofRen_id : ofRen id = Term.var := rfl
 
 theorem ofRen_upr: ofRen (upr ξ) = up (ofRen ξ) := by
-  ext ⟨⟩ <;> simp [ofRen, upr, up, snoc, rename]; sorry
+  ext ⟨⟩ <;> simp [ofRen, upr, up, snoc, rename]
 
-theorem rename_eq_subst_ofRen (ξ : Nat → Nat) : rename ξ = subst (ofRen ξ) := by sorry
-  -- ext t
-  -- induction t generalizing ξ <;> dsimp [rename, subst]
-  -- case bvar => simp [ofRen]
-  -- all_goals grind [ofRen_upr]
+theorem rename_eq_subst_ofRen (ξ : Nat → Nat) : rename ξ = subst (ofRen ξ) := by
+  ext t
+  induction t generalizing ξ <;> simp [rename, subst]
+  case var => simp [ofRen]
+  all_goals grind [ofRen_upr]
 
 /-- Compose two substitutions.
 ```
@@ -93,13 +105,89 @@ def comp (σ τ : Nat → Term) : Nat → Term :=
   subst σ ∘ τ
 
 @[simp]
-theorem bvar_comp (σ : Nat → Term) : comp Term.var σ = σ := by
+theorem var_comp (σ : Nat → Term) : comp Term.var σ = σ := by
   ext i; simp [comp]
 
 @[simp]
-theorem comp_bvar (σ : Nat → Term) : comp σ Term.var = σ := by
-  ext i; simp [comp, subst]; sorry
+theorem comp_var (σ : Nat → Term) : comp σ Term.var = σ := by
+  ext i; simp [comp, subst]
 
 theorem up_comp_ren_sb (ξ : Nat → Nat) (σ : Nat → Term) :
     up (σ ∘ ξ) = up σ ∘ upr ξ := by
   ext ⟨⟩ <;> (unfold up; dsimp [snoc, upr])
+
+theorem rename_subst (σ ξ) (t : Term) : (t.rename ξ).subst σ = t.subst (σ ∘ ξ) := by
+  induction t generalizing σ ξ
+  all_goals try grind [rename, subst, up_comp_ren_sb, map_id''_mem, app.injEq, List.map_inj_left]
+
+theorem up_comp_sb_ren (σ : Nat → Term) (ξ : Nat → Nat) :
+    up (rename ξ ∘ σ) = rename (upr ξ) ∘ up σ := by
+  ext ⟨⟩ <;> (unfold up; simp [snoc, rename, upr])
+  conv => lhs; rw [rename_eq_subst_ofRen, rename_subst]
+  conv => rhs; rw [rename_eq_subst_ofRen, rename_subst]
+  rfl
+
+theorem subst_rename (ξ σ) (t : Term) :
+    (t.subst σ).rename ξ = t.subst (rename ξ ∘ σ) := by
+  induction t generalizing ξ σ
+  all_goals grind [subst, rename, up_comp_sb_ren, map_id''_mem, app.injEq, List.map_inj_left]
+
+theorem up_comp (σ τ : Nat → Term) :
+    up (comp σ τ) = comp (up σ) (up τ) := by
+  ext ⟨⟩ <;> simp [up, comp, snoc]
+  simp [subst_rename, rename_subst]; congr
+
+theorem subst_subst (σ τ : Nat → Term) (t : Term) :
+    (t.subst τ).subst σ = t.subst (comp σ τ) := by
+  induction t generalizing σ τ
+  case var => simp [subst, comp]
+  all_goals grind [subst, up_comp, map_id''_mem, app.injEq, List.map_inj_left]
+
+theorem comp_assoc (σ τ ρ : Nat → Term) : comp σ (comp τ ρ) = comp (comp σ τ) ρ := by
+  ext i
+  conv => rhs; enter [0]; unfold comp
+  dsimp; rw [← subst_subst]; dsimp [comp]
+
+theorem comp_snoc (σ τ : Nat → Term) (t : Term) :
+    comp σ (snoc τ t) = snoc (comp σ τ) (t.subst σ) := by
+  ext ⟨⟩ <;> dsimp [comp, snoc]
+
+
+/-- The weakening substitution.
+```
+Γ ⊢ A
+------------
+Γ.A ⊢ ↑ : Γ
+``` -/
+def wk : Nat → Term :=
+  ofRen Nat.succ
+
+@[simp]
+theorem ofRen_succ : ofRen Nat.succ = wk := rfl
+
+theorem up_eq_snoc (σ : Nat → Term) : up σ = snoc (comp wk σ) (.var 0) := by
+  ext i; unfold up comp; congr 1; ext j
+  rw [rename_eq_subst_ofRen]; congr 1
+
+@[simp]
+theorem snoc_comp_wk (σ : Nat → Term) (t) : comp (snoc σ t) wk = σ := by
+  ext ⟨⟩ <;> simp [comp, snoc, wk, ofRen, subst, -ofRen_succ]
+
+@[simp]
+theorem snoc_wk_zero : snoc wk (Term.var 0) = Term.var := by
+  ext ⟨⟩ <;> dsimp [snoc, wk, ofRen, -ofRen_succ]
+
+theorem snoc_comp_wk_succ (σ : Nat → Term) (n) :
+    snoc (comp wk σ) (var (n + 1)) = comp wk (snoc σ (var n)) := by
+  ext ⟨⟩ <;> simp [comp, snoc, wk, -ofRen_succ, subst, ofRen]
+
+/-- A substitution that instantiates one binder.
+```
+Γ ⊢ t : A
+--------------
+Γ ⊢ id.t : Γ.A
+``` -/
+def toSb (t : Term) : Nat → Term :=
+  snoc Term.var t
+
+end IR.Term
